SkLean/Candidates2.lean
@@ -1,0 +1,27 @@
+import SkLean.Ast2
+
+/-
+# Hierarchied SK Reducibility Candidates
+
+-/
+
+inductive is_candidate_n : ℕ → Expr → Expr → Prop
+  | stuck : (¬(∃ e', is_eval_once e e')) → is_candidate_n 0 e e
+  | succ  : is_eval_once e e'
+    → e_final.max_universe < e.max_universe
+    → is_candidate_n n e' e_final
+    → is_candidate_n n.succ e e_final
+
+namespace is_candidate_for
+
+lemma imp_judgment : is_candidate_for e t → valid_judgment e t := by
+  intro h_r
+  induction h_r
+  case stuck t' h_step h =>
+    exact h
+  case step e' t' h_beq h_u =>
+    
+    sorry
+
+end is_candidate_for
+
