SkLean/Sn2.lean
@@ -1,28 +1,31 @@
 import SkLean.Ast2
+import SkLean.Typing2
 import Mathlib.Tactic
 
 inductive sn : Expr → Prop
   | hard : (∀ e', is_eval_once e e' → sn e') → sn e
 
-lemma sn_call_k : sn SKM[(((K n) x) y)] → sn x := by
+namespace sn
+
+lemma call_k : sn SKM[(((K n) x) y)] → sn x := by
   intro h_sn
   match h_sn with
     | .hard h_step =>
       exact h_step x (by apply is_eval_once.k)
 
-lemma sn_call_s : sn SKM[((((S n) x) y) z)] → sn SKM[((x z) (y z))] := by
+lemma call_s : sn SKM[((((S n) x) y) z)] → sn SKM[((x z) (y z))] := by
   intro h_sn
   match h_sn with
     | .hard h_step =>
       exact h_step SKM[((x z) (y z))] (by apply is_eval_once.s)
 
-lemma sn_call_m : sn SKM[(M n e)] → valid_judgment e t → sn t := by
+lemma call_m : sn SKM[((M e.max_universe.succ) e)] → valid_judgment e t → sn t := by
   intro h_sn h_t
   match h_sn with
     | .hard h_step =>
-      exact h_step t (by apply is_eval_once.m; exact h_t)
+      exact h_step t (by apply is_eval_once.m_final; exact h_t)
 
-lemma sn_preserved : sn e → is_eval_once e e' → sn e' := by
+lemma preserved : sn e → is_eval_once e e' → sn e' := by
   intro h_sn h_eval
   cases e
   cases h_eval
@@ -33,47 +36,24 @@ lemma sn_preserved : sn e → is_eval_once e e' → sn e' := by
       | .hard h_step =>
         exact h_step e' h_eval
 
-lemma sn_imp_n_steps_eval_normal (e : Expr) : valid_judgment e t → sn e → ∃ n e', is_normal_n n e e' := by
+lemma imp_n_steps_eval_normal (e : Expr) : valid_judgment e t → sn e → ∃ n e', is_normal_n n e e' := by
   intro h_t h_sn
-  induction h_sn
-  case hard e' h_step h_eval' =>
-    match e' with
-      | SKM[M n] =>
-        use 0
-        use SKM[M n]
-        apply m_stuck
-      | SKM[K n] =>
-        use 0
-        use SKM[K n]
-        apply k_stuck
-      | SKM[S n] =>
-        use 0
-        use SKM[S n]
-        apply s_stuck
-      | SKM[(((K n) x) y)] =>
-        have h_x_sn := h_step x (by apply is_eval_once.k)
-        have ⟨n_norm, norm_x, h_norm_x⟩ := h_eval' x (by apply is_eval_once.k) (by sorry)
-        use n_norm.succ
-        use norm_x
-        apply is_normal_n.succ
-        apply is_eval_once.k
-        exact h_norm_x
-      | SKM[((((S n) x) y) z)] =>
-        have h_eval_sn := h_step SKM[((x z) (y z))] (by apply is_eval_once.s)
-        have ⟨n_norm, norm_eval, h_norm_eval⟩ := h_eval' SKM[((x z) (y z))] (by apply is_eval_once.s) sorry
-        use n_norm.succ
-        use norm_eval
-        apply is_normal_n.succ
-        apply is_eval_once.s
-        exact h_norm_eval
-      | SKM[(M n e)] =>
-        have h_eval_sn := h_step t (by apply is_eval_once.m)
-        have ⟨n_norm, norm_eval, h_norm_eval⟩ := h_eval' SKM[((x z) (y z))] (by apply is_eval_once.s) sorry
-        use n_norm.succ
-        use norm_eval
-        apply is_normal_n.succ
-        apply is_eval_once.s
-        exact h_norm_eval
-        sorry
-      | SKM[(lhs rhs)] => sorry
+  induction e
+  case m n =>
+    use 0
+    use SKM[M n]
+    apply is_normal_n.m_stuck
+  case k n =>
+    use 0
+    use SKM[K n]
+    apply is_normal_n.k_stuck
+  case s n =>
+    use 0
+    use SKM[S n]
+    apply is_normal_n.s_stuck
+  case call lhs rhs h₁ h₂ =>
+    cases h_t
+    case call h₁' h₂' h₃' =>
+      cases h₁'
 
+end sn
