SkLean/Typing2.lean
@@ -2,7 +2,7 @@ import SkLean.Ast2
 
 namespace valid_judgment
 
-lemma eval_preserves_judgment_hard : ∀ e e' t, valid_judgment e t → is_eval_once e e' → valid_judgment e' t := by
+lemma preserved : ∀ e e' t, valid_judgment e t → is_eval_once e e' → valid_judgment e' t := by
   intro e e' t h_t h_eval
   induction h_t
   cases h_eval
